moved out lemmas

concurrency/sync_preds.v
@@ -60,6 +60,8 @@ Definition LKspec_ext (R: pred rmap) : spec :=
 Definition LK_at R sh :=
   LKspec_ext R (Share.unrel Share.Lsh sh) (Share.unrel Share.Rsh sh).
 
+(** * Results related to resouce_decay *)
+
 Lemma resource_decay_LK {b phi phi' loc rsh sh n pp} :
   resource_decay b phi phi' ->
   phi @ loc = YES rsh sh (LK n) pp ->
@@ -331,6 +333,8 @@ Proof.
     repeat eexists.
 Qed.
 
+(** * Results related to aging  *)
+
 Lemma app_pred_age {R} {phi phi' : rmap} :
   age phi phi' ->
   app_pred R phi ->
@@ -520,4 +524,497 @@ Proof.
   destruct (age1 jm) as [jm'|] eqn:e.
   - rewrite (age1_juicy_mem_Some _ _ e). easy.
   - rewrite (age1_juicy_mem_None1 _ e). easy.
+Qed.
+
+(** * Results on cl_step *)
+
+Lemma cl_step_decay ge c m c' m' : @cl_step ge c m c' m' -> @decay m m'.
+Proof.
+  intros step.
+  induction step
+    as [ ve te k m a1 a2 b ofs v2 v m' H H0 H1 H2 ASS | |
+         ve te k m optid a al tyagrs tyres cc vf vargs f m'  ve' le' H H0 H1 H2 H3 H4 NRV ALLOC H6 
+         | | | | | | | | | f ve te optexp optid k m v' m' ve' te'' k' H H0 FREE H2 H3 | | | ];
+    try apply decay_refl || apply IHstep.
+  
+  - (* assign: no change in permission *)
+    intros b' ofs'.
+    split.
+    + inversion ASS as [v0 chunk m'0 H3 BAD H5 H6 | b'0 ofs'0 bytes m'0 H3 H4 H5 H6 H7 BAD H9 H10]; subst.
+      -- pose proof storev_valid_block_2 _ _ _ _ _ BAD b'. tauto.
+      -- pose proof Mem.storebytes_valid_block_2 _ _ _ _ _ BAD b'. tauto.
+    + intros V; right; intros kind.
+      (* destruct m as [c acc nb max no def]. simpl in *. *)
+      inversion ASS as [v0 chunk m'0 H3 STO H5 H6 | b'0 ofs'0 bytes m'0 H3 H4 H5 H6 H7 STO H9 H10]; subst.
+      -- simpl in *.
+         Transparent Mem.store.
+         unfold Mem.store in *; simpl in *.
+         destruct (Mem.valid_access_dec m chunk b (Int.unsigned ofs) Writable).
+         2:discriminate.
+         injection STO as <-. simpl.
+         reflexivity.
+      -- Transparent Mem.storebytes.
+         unfold Mem.storebytes in *.
+         destruct (Mem.range_perm_dec
+                     m b (Int.unsigned ofs)
+                     (Int.unsigned ofs + Z.of_nat (Datatypes.length bytes)) Cur Writable).
+         2:discriminate.
+         injection STO as <-. simpl.
+         reflexivity.
+  
+  - (* internal call : allocations *)
+    clear -ALLOC.
+    induction ALLOC. now apply decay_refl.
+    apply decay_trans with m1. 3:apply IHALLOC.
+    
+    + clear -H.
+      Transparent Mem.alloc.
+      unfold Mem.alloc in *.
+      injection H as <- <-.
+      intros b V.
+      unfold Mem.valid_block in *. simpl.
+      apply Coqlib.Plt_trans_succ, V.
+      
+    + clear -H.
+      unfold Mem.alloc in *.
+      injection H as E <-.
+      intros b ofs.
+      split.
+      * intros N V.
+        subst m1.
+        simpl in *.
+        rewrite PMap.gsspec.
+        unfold Mem.valid_block in *; simpl in *.
+        if_tac; subst; auto.
+        -- if_tac; auto.
+        -- destruct N.
+           apply Coqlib.Plt_succ_inv in V.
+           tauto.
+      * intros V.
+        right.
+        intros k.
+        subst.
+        simpl.
+        rewrite PMap.gsspec.
+        if_tac.
+        -- subst b. inversion V. rewrite Pos.compare_lt_iff in *. edestruct Pos.lt_irrefl; eauto.
+        -- reflexivity.
+  
+  - (* return: free_list *)
+    revert FREE; clear.
+    generalize (blocks_of_env ge ve); intros l.
+    revert m m'; induction l as [| [[b o] o'] l IHl]; intros m m'' E.
+    + simpl. injection E as <- ; apply decay_refl.
+    + simpl in E.
+      destruct (Mem.free m b o o') as [m' |] eqn:F.
+      2:discriminate.
+      specialize (IHl _ _ E).
+      Transparent Mem.free.
+      unfold Mem.free in *.
+      if_tac in F. rename H into G.
+      2:discriminate.
+      apply decay_trans with m'. 3:now apply IHl.
+      * injection F as <-.
+        intros.
+        unfold Mem.unchecked_free, Mem.valid_block in *.
+        simpl in *.
+        assumption.
+      
+      * injection F as <-.
+        clear -G.
+        unfold Mem.unchecked_free in *.
+        intros b' ofs; simpl. unfold Mem.valid_block; simpl.
+        split.
+        tauto.
+        intros V.
+        rewrite PMap.gsspec.
+        if_tac; auto. subst b'.
+        hnf in G.
+        destruct (Coqlib.proj_sumbool (Coqlib.zle o ofs)&&Coqlib.proj_sumbool (Coqlib.zlt ofs o')) eqn:E.
+        2: now auto.
+        left. split; auto.
+        destruct m as [co acc nb max noa def] eqn:Em; simpl in *.
+        unfold Mem.perm in G; simpl in *.
+        specialize (G ofs).
+        cut (acc !! b ofs Cur = Some Freeable). {
+          destruct k; auto.
+          pose proof Mem.access_max m b ofs as M.
+          subst m; simpl in M.
+          intros A; rewrite A in M.
+          destruct (acc !! b ofs Max) as [ [] | ]; inversion M; auto.
+        }
+        assert (R: (o <= ofs < o')%Z). {
+          rewrite andb_true_iff in *. destruct E as [E F].
+          apply Coqlib.proj_sumbool_true in E.
+          apply Coqlib.proj_sumbool_true in F.
+          auto.
+        }
+        autospec G.
+        destruct (acc !! b ofs Cur) as [ [] | ]; inversion G; auto.
+Qed.
+
+Lemma cl_step_unchanged_on ge c m c' m' b ofs :
+  @cl_step ge c m c' m' ->
+  Mem.valid_block m b ->
+  ~ Mem.perm m b ofs Cur Writable ->
+  Maps.ZMap.get ofs (Maps.PMap.get b (Mem.mem_contents m)) =
+  Maps.ZMap.get ofs (Maps.PMap.get b (Mem.mem_contents m')).
+Proof.
+  intros step.
+  induction step
+    as [ ve te k m a1 a2 b0 ofs0 v2 v m' H H0 H1 H2 ASS | |
+         ve te k m optid a al tyagrs tyres cc vf vargs f m'  ve' le' H H0 H1 H2 H3 H4 NRV ALLOC H6 
+         | | | | | | | | | f ve te optexp optid k m v' m' ve' te'' k' H H0 FREE H2 H3 | | | ];
+    intros V NW; auto.
+  
+  - (* assign: some things are updated, but not the chunk in non-writable permission *)
+    inversion ASS; subst.
+    + inversion H4.
+      unfold Mem.store in *.
+      destruct (Mem.valid_access_dec m chunk b0 (Int.unsigned ofs0) Writable); [|discriminate].
+      injection H6 as <- ; clear ASS H4.
+      simpl.
+      destruct (eq_dec b b0) as [e|n]; swap 1 2.
+      * rewrite PMap.gso; auto.
+      * subst b0. rewrite PMap.gss.
+        generalize ((Mem.mem_contents m) !! b); intros t.
+        destruct v0 as [v0 align].
+        specialize (v0 ofs).
+        {
+          destruct (adr_range_dec (b, Int.unsigned ofs0) (size_chunk chunk) (b, ofs)) as [a|a].
+          - simpl in a; destruct a as [_ a].
+            autospec v0.
+            tauto.
+          - simpl in a.
+            symmetry.
+            apply Mem.setN_outside.
+            rewrite encode_val_length.
+            replace (Z_of_nat (size_chunk_nat chunk)) with (size_chunk chunk); swap 1 2.
+            { unfold size_chunk_nat in *. rewrite Z2Nat.id; auto. destruct chunk; simpl; omega. }
+            assert (a' : ~ (Int.unsigned ofs0 <= ofs < Int.unsigned ofs0 + size_chunk chunk)%Z) by intuition.
+            revert a'; clear.
+            generalize (Int.unsigned ofs0).
+            generalize (size_chunk chunk).
+            intros.
+            omega.
+        }
+    
+    + (* still the case of assignment (copying) *)
+      unfold Mem.storebytes in *.
+      destruct (Mem.range_perm_dec m b0 (Int.unsigned ofs0) (Int.unsigned ofs0 + Z.of_nat (Datatypes.length bytes)) Cur Writable); [ | discriminate ].
+      injection H8 as <-; clear ASS; simpl.
+      destruct (eq_dec b b0) as [e|n]; swap 1 2.
+      * rewrite PMap.gso; auto.
+      * subst b0. rewrite PMap.gss.
+        generalize ((Mem.mem_contents m) !! b); intros t.
+        specialize (r ofs).
+        {
+          destruct (adr_range_dec (b, Int.unsigned ofs0) (Z.of_nat (Datatypes.length bytes)) (b, ofs)) as [a|a].
+          - simpl in a; destruct a as [_ a].
+            autospec r.
+            tauto.
+          - simpl in a.
+            symmetry.
+            apply Mem.setN_outside.
+            assert (a' : ~ (Int.unsigned ofs0 <= ofs < Int.unsigned ofs0 + Z.of_nat (Datatypes.length bytes))%Z) by intuition.
+            revert a'; clear.
+            generalize (Int.unsigned ofs0).
+            intros.
+            omega.
+        }
+  
+  - (* internal call : things are allocated -- each time in a new block *)
+    clear -V ALLOC.
+    induction ALLOC. easy.
+    rewrite <-IHALLOC; swap 1 2.
+    + unfold Mem.alloc in *.
+      injection H as <- <-.
+      unfold Mem.valid_block in *.
+      simpl.
+      apply Plt_trans_succ.
+      auto.
+    + clear IHALLOC.
+      unfold Mem.alloc in *.
+      injection H as <- <- . simpl.
+      f_equal.
+      rewrite PMap.gso. auto.
+      unfold Mem.valid_block in *.
+      auto with *.
+  
+  - (* return: free_list *)
+    revert FREE NW V; clear.
+    generalize (blocks_of_env ge ve); intros l.
+    revert m m'; induction l as [| [[b' o] o'] l IHl]; intros m m'' E NW V.
+    + simpl. injection E as <- . easy.
+    + simpl in E.
+      destruct (Mem.free m b' o o') as [m' |] eqn:F.
+      2:discriminate.
+      specialize (IHl _ _ E).
+      unfold Mem.free in *.
+      if_tac in F. 2:discriminate.
+      injection F as <- .
+      rewrite <-IHl. easy.
+      * unfold Mem.perm in *.
+        unfold Mem.unchecked_free.
+        simpl.
+        rewrite PMap.gsspec.
+        if_tac; [ | easy ].
+        subst.
+        unfold Mem.range_perm in *.
+        destruct (zle o ofs); auto.
+        destruct (zlt ofs o'); simpl; auto.
+      * unfold Mem.unchecked_free, Mem.valid_block; simpl. auto.
+Qed.
+
+
+(** * Results related to machine predicates *)
+   
+(* Instantiation of modules *)
+Import THE_JUICY_MACHINE.
+Import JSEM.
+Module Machine :=THE_JUICY_MACHINE.JTP.
+Definition schedule := SCH.schedule.
+Import JuicyMachineLemmas.
+Import ThreadPool.
+
+Lemma same_locks_juicyLocks_in_lockSet phi phi' lset :
+  same_locks phi phi' ->
+  juicyLocks_in_lockSet lset phi ->
+  juicyLocks_in_lockSet lset phi'.
+Proof.
+  intros SL IN loc sh psh P n E.
+  destruct (SL loc) as [_ (rsh & sh' & n' & pp & E')].
+  { rewrite E. repeat eexists. }
+  apply (IN loc _ _ _ _ E').
+Qed.
+
+Lemma resource_decay_lockSet_in_juicyLocks b phi phi' lset :
+  resource_decay b phi phi' ->
+  lockSet_block_bound lset b ->
+  lockSet_in_juicyLocks lset phi ->
+  lockSet_in_juicyLocks lset phi'.
+Proof.
+  intros RD LB IN loc IT.
+  destruct (IN _ IT) as (rsh & sh & pp & E).
+  (* assert (SL : same_locks phi phi') by (eapply resource_decay_same_locks; eauto). *)
+  assert (SL : same_locks_sized phi phi') by (eapply resource_decay_same_locks_sized; eauto).
+  destruct (SL loc LKSIZE) as [(rsh' & sh' & pp' &  E') _].
+  { rewrite E. exists rsh, sh, pp. reflexivity. }
+  destruct RD as [L RD].
+  destruct (RD loc) as [NN [R|[R|[[P [v R]]|R]]]].
+  + rewrite E in R. simpl in R; rewrite <- R.
+    eauto.
+  + rewrite E in R. destruct R as (sh'' & v & v' & R & H). discriminate.
+  + specialize (LB loc).
+    cut (fst loc < b)%positive. now intro; exfalso; eauto.
+    apply LB. destruct (AMap.find (elt:=option rmap) loc lset).
+    * apply I.
+    * inversion IT.
+  + destruct R as (v & v' & R & N').
+    rewrite E'.
+    exists rsh', sh', pp'.
+    eauto.
+Qed.
+
+Lemma lockSet_Writable_lockSet_block_bound m lset  :
+  lockSet_Writable lset m ->
+  lockSet_block_bound lset (Mem.nextblock m).
+Proof.
+  simpl; intros LW.
+  intros (b, ofs) IN; simpl.
+  specialize (LW b ofs).
+  destruct (AMap.find (elt:=option rmap) (b, ofs) lset). 2:inversion IN.
+  specialize (LW eq_refl).
+  cut (~ ~ (b < Mem.nextblock m)%positive). zify. omega. intros L.
+  specialize (LW ofs).
+  assert (Intv.In ofs (ofs, (ofs + LKSIZE)%Z)).
+  { split; simpl; unfold LKSIZE in *; simpl; omega. }
+  autospec LW.
+  rewrite (Mem.nextblock_noaccess _ _ ofs Max L) in LW.
+  inversion LW.
+Qed.
+
+Lemma join_all_age_updThread_level tp i (cnti : ThreadPool.containsThread tp i) c phi Phi :
+  join_all (age_tp_to (level phi) (ThreadPool.updThread cnti c phi)) Phi ->
+  level Phi = level phi.
+Proof.
+  intros J; symmetry.
+  remember (level phi) as n.
+  rewrite <- (level_age_to n phi). 2:omega.
+  apply rmap_join_sub_eq_level.
+  assert (cnti' : containsThread (updThread cnti c phi) i) by eauto with *.
+  rewrite (@cnt_age _ _ n) in cnti'.
+  pose proof compatible_threadRes_sub cnti' J as H.
+  unshelve erewrite <-getThreadR_age in H; eauto with *.
+  rewrite gssThreadRes in H.
+  apply H.
+Qed.
+
+Lemma join_all_level_lset tp Phi l phi :
+  join_all tp Phi ->
+  AMap.find l (lset tp) = SSome phi ->
+  level phi = level Phi.
+Proof.
+  intros J F.
+  apply rmap_join_sub_eq_level.
+  eapply compatible_lockRes_sub; eauto.
+Qed.
+
+Lemma lset_range_perm m tp b ofs
+  (compat : mem_compatible tp m)
+  (Efind : AMap.find (elt:=option rmap) (b, ofs) (lset tp) <> None) :
+  Mem.range_perm
+    (restrPermMap (mem_compatible_locks_ltwritable compat))
+    b ofs (ofs + size_chunk Mint32) Cur Writable.
+Proof.
+  unfold Mem.range_perm in *.
+  intros ofs0 range.
+  unfold Mem.perm in *.
+  pose proof restrPermMap_Cur as R.
+  unfold permission_at in *.
+  rewrite R.
+  erewrite lockSet_spec_2.
+  + constructor.
+  + eauto.
+  + unfold lockRes in *.
+    unfold lockGuts in *.
+    unfold LocksAndResources.lock_info in *.
+    destruct (AMap.find (elt:=option rmap) (b, ofs) (lset tp)).
+    * reflexivity.
+    * tauto.
+Qed.
+
+Lemma age_to_updThread i tp n c phi cnti cnti' :
+  age_tp_to n (@updThread i tp cnti c phi) =
+  @updThread i (age_tp_to n tp) cnti' c (age_to n phi).
+Proof.
+  destruct tp; simpl.
+  unfold updThread in *; simpl.
+  f_equal. extensionality j.
+  unfold "oo".
+  do 2 match goal with
+         |- context [if ?a then _ else _] =>
+         let E := fresh "E" in
+         destruct a eqn:E
+       end.
+  all:auto.
+  all:cut (true = false); [ congruence | ].
+  all:rewrite <-E, <-E0; repeat f_equal; apply proof_irr.
+Qed.
+
+Lemma lset_age_tp_to n tp :
+  lset (age_tp_to n tp) = AMap.map (option_map (age_to n)) (lset tp).
+Proof.
+  destruct tp; reflexivity.
+Qed.
+
+Lemma getThreadC_fun i tp cnti cnti' x y :
+  @getThreadC i tp cnti = x ->
+  @getThreadC i tp cnti' = y ->
+  x = y.
+Proof.
+  intros <- <-.
+  unfold getThreadC, containsThread in *.
+  repeat f_equal.
+  apply proof_irr.
+Qed.
+
+Lemma getThreadR_fun i tp cnti cnti' x y :
+  @getThreadR i tp cnti = x ->
+  @getThreadR i tp cnti' = y ->
+  x = y.
+Proof.
+  intros <- <-.
+  unfold getThreadR, containsThread in *.
+  repeat f_equal.
+  apply proof_irr.
+Qed.
+
+Lemma lockSet_Writable_age n tp m :
+  lockSet_Writable (lset tp) m ->
+  lockSet_Writable (lset (age_tp_to n tp)) m.
+Proof.
+  rewrite lset_age_tp_to.
+  intros L b ofs E ofs0 range.
+  refine(L b ofs _ ofs0 range).
+  exact_eq E; f_equal.
+  apply isSome_find_map.
+Qed.
+
+Lemma juicyLocks_in_lockSet_age n tp phi :
+  juicyLocks_in_lockSet (lset tp) phi ->
+  juicyLocks_in_lockSet (lset (age_tp_to n tp)) (age_to n phi).
+Proof.
+  rewrite lset_age_tp_to.
+  intros L loc sh sh' pp z E.
+  pattern pp in E.
+  pose proof ex_intro _ pp E as H.
+  pattern (age_to n phi) in H.
+  rewrite <-rewrite_age_to in H; swap 1 2.
+  - intros; eapply age1_YES'; auto.
+  - destruct H as (pp', E').
+    specialize (L loc sh sh' pp' z E').
+    exact_eq L; f_equal.
+    symmetry.
+    apply isSome_find_map.
+Qed.
+
+Lemma lockSet_in_juicyLocks_age n tp phi :
+  lockSet_in_juicyLocks (lset tp) phi ->
+  lockSet_in_juicyLocks (lset (age_tp_to n tp)) (age_to n phi).
+Proof.
+  rewrite lset_age_tp_to.
+  intros L loc E.
+  rewrite isSome_find_map in E.
+  specialize (L loc E).
+  destruct L as (sh & sh' & L). exists sh, sh'.
+  pattern (age_to n phi).
+  rewrite <-rewrite_age_to. easy.
+  intros; eapply age1_YES'; auto.
+Qed.
+
+Definition same_except_cur (m m' : Mem.mem) :=
+  Mem.mem_contents m = Mem.mem_contents m' /\
+  max_access_at m = max_access_at m' /\
+  Mem.nextblock m = Mem.nextblock m'.
+
+Lemma mem_cohere_same_except_cur m m' phi :
+  same_except_cur m m' ->
+  mem_cohere' m phi ->
+  mem_cohere' m' phi.
+Proof.
+  intros (ECo & EMa & EN) [Co Ac Ma N]; constructor.
+  - hnf in *.
+    unfold contents_at in *.
+    rewrite <-ECo. auto.
+  - unfold access_cohere' in *.
+    unfold max_access_at in *.
+    intros.
+    apply equal_f with (x := loc) in EMa.
+    rewrite <-EMa.
+    auto.
+  - unfold max_access_cohere in *. intros loc.
+    apply equal_f with (x := loc) in EMa.
+    rewrite <-EMa, <-EN.
+    apply Ma.
+  - hnf in *. rewrite <-EN.
+    auto.
+Qed.
+  
+Lemma mem_compatible_with_same_except_cur tp m m' phi :
+  same_except_cur m m' ->
+  mem_compatible_with tp m phi ->
+  mem_compatible_with tp m' phi.
+Proof.
+  intros E [J AC LW LJ JL]; constructor; auto.
+  - eapply mem_cohere_same_except_cur. apply E. apply AC.
+  - destruct E as (ECo & EMa & EN).
+    intros b ofs Ef ofs0 Ran.
+    specialize (LW b ofs Ef ofs0 Ran).
+    unfold max_access_cohere in *.
+    apply equal_f with (x := (b, ofs0)) in EMa.
+    unfold max_access_at in *.
+    simpl in *.
+    rewrite <-EMa.
+    auto.
 Qed.
